wip for proving equivalence of semantics of operators

cfrontend/BeePL.v
@@ -180,214 +180,217 @@ match xs with
 end.
 
 (***** Semantics of unary operators *****)
-Definition sem_notbool (v : value) : option value :=
-match v with 
-| Vunit => None 
-| Vint i => None
-| Vuint i => None 
-| Vbool b => Some (of_bool (negb b)) 
-| Vloc l => None
+Definition sem_notbool (v : value) (t : type) : option value :=
+match v,t with 
+| Vunit, (Ptype Tunit) => None 
+| Vint i, (Ptype Tint) => None
+| Vuint i, (Ptype Tuint) => None 
+| Vbool b, (Ptype Tbool) => Some (of_bool (negb b)) 
+| Vloc l, (Reftype _ (Bprim Tint))  => None
+| _, _ => None
 end.
 
-
-Definition sem_notint (v : value) : option value :=
-match v with 
-| Vunit => None 
-| Vint i => Some (of_int (Int.not i)) 
-| Vuint i => Some (of_int (Int.not i))
-| Vbool b => None 
-| Vloc l => None 
+Definition sem_notint (v : value) (t : type) : option value :=
+match v,t with 
+| Vunit, (Ptype Tunit) => None 
+| Vint i, (Ptype Tint) => Some (of_int (Int.not i)) 
+| Vuint i, (Ptype Tuint) => Some (of_int (Int.not i))
+| Vbool b, (Ptype Tbool) => None 
+| Vloc l, (Reftype _ (Bprim Tint)) => None 
+| _, _ => None
 end.
 
-Definition sem_neg (v : value) : option value :=
-match v with 
-| Vunit => None 
-| Vint i => Some (of_int (Int.neg i)) 
-| Vuint i => Some (of_int (Int.neg i))
-| Vbool b => None 
-| Vloc l => None 
+Definition sem_neg (v : value) (t : type) : option value :=
+match v,t with 
+| Vunit, (Ptype Tunit) => None 
+| Vint i, (Ptype Tint) => Some (of_int (Int.neg i)) 
+| Vuint i, (Ptype Tuint) => Some (of_int (Int.neg i))
+| Vbool b, (Ptype Tbool) => None 
+| Vloc l, (Reftype _ (Bprim Tint)) => None
+| _, _ => None 
 end.
 
-Definition sem_unary_operation (op : uop) (v : value) : option value :=
+Definition sem_unary_operation (op : uop) (v : value) (t : type) : option value :=
 match op with 
-| Notbool => sem_notbool v 
-| Notint => sem_notint v
-| Neg => sem_neg v
+| Notbool => sem_notbool v t
+| Notint => sem_notint v t
+| Neg => sem_neg v t
 end.
 
 
 (***** Semantics of binary operators *****)
 (* Addition: Integer overflow is taken care in the definition of int 
    Example : 4 bit (15 is the max) : 15 + 1 wraps around and produces 0 *)
-Definition sem_plus (v1 : value) (v2 : value) : option value :=
-match v1, v2 with 
-| Vunit, Vunit => None
-| Vbool b1, Vbool b2 => None 
-| Vint i1, Vint i2 => Some (of_int (Int.add i1 i2)) 
-| Vuint i1, Vuint i2 => Some (of_int (Int.add i1 i2))
-| Vloc l1, Vloc l2 => None 
-| _, _ => None
+Definition sem_plus (v1 : value) (v2 : value) (t1 : type) (t2 : type) : option value :=
+match v1, v2, t1, t2 with 
+| Vunit, Vunit, (Ptype Tunit), (Ptype Tunit) => None
+| Vbool b1, Vbool b2, (Ptype Tbool), (Ptype Tbool) => None 
+| Vint i1, Vint i2, (Ptype Tint), (Ptype Tint) => Some (of_int (Int.add i1 i2)) 
+| Vuint i1, Vuint i2, (Ptype Tuint), (Ptype Tunit) => Some (of_int (Int.add i1 i2))
+| Vloc l1, Vloc l2, (Reftype _ (Bprim Tint)), (Reftype _ (Bprim Tint)) => None 
+| _, _, _, _ => None
 end.
 
-Definition sem_minus (v1 : value) (v2 : value) : option value :=
-match v1, v2 with 
-| Vunit, Vunit => None
-| Vbool b1, Vbool b2 => None 
-| Vint i1, Vint i2 => Some (of_int (Int.sub i1 i2)) 
-| Vuint i1, Vuint i2 => Some (of_int (Int.sub i1 i2))
-| Vloc l1, Vloc l2 => None 
-| _, _ => None
+Definition sem_minus (v1 : value) (v2 : value) (t1 : type) (t2 : type) : option value :=
+match v1, v2, t1, t2 with 
+| Vunit, Vunit, (Ptype Tunit), (Ptype Tunit) => None
+| Vbool b1, Vbool b2, (Ptype Tbool), (Ptype Tbool) => None 
+| Vint i1, Vint i2, (Ptype Tint), (Ptype Tint) => Some (of_int (Int.sub i1 i2)) 
+| Vuint i1, Vuint i2, (Ptype Tuint), (Ptype Tuint) => Some (of_int (Int.sub i1 i2))
+| Vloc l1, Vloc l2, (Reftype _ (Bprim Tint)), (Reftype _ (Bprim Tint)) => None 
+| _, _, _, _ => None
 end.
 
-Definition sem_mult (v1 : value) (v2 : value) : option value :=
-match v1, v2 with 
-| Vunit, Vunit => None
-| Vbool b1, Vbool b2 => None 
-| Vint i1, Vint i2 => Some (of_int (Int.mul i1 i2)) 
-| Vuint i1, Vuint i2 => Some (of_int (Int.mul i1 i2))
-| Vloc l1, Vloc l2 => None 
-| _, _ => None
+Definition sem_mult (v1 : value) (v2 : value) (t1 : type) (t2 : type) : option value :=
+match v1, v2, t1, t2 with 
+| Vunit, Vunit, (Ptype Tunit), (Ptype Tunit) => None
+| Vbool b1, Vbool b2, (Ptype Tbool), (Ptype Tbool) => None 
+| Vint i1, Vint i2, (Ptype Tint), (Ptype Tint) => Some (of_int (Int.mul i1 i2)) 
+| Vuint i1, Vuint i2, (Ptype Tuint), (Ptype Tuint) => Some (of_int (Int.mul i1 i2))
+| Vloc l1, Vloc l2, (Reftype _ (Bprim Tint)), (Reftype _ (Bprim Tint)) => None 
+| _, _, _, _ => None
 end.
 
-Definition sem_div (v1 : value) (v2 : value) : option value :=
-match v1, v2 with 
-| Vunit, Vunit => None
-| Vbool b1, Vbool b2 => None 
-| Vint i1, Vint i2 => if (Int.eq i2 Int.zero) || (Int.eq i1 (Int.repr Int.min_signed) && Int.eq i2 Int.mone) (* -128/-1 *)
+Definition sem_div (v1 : value) (v2 : value) (t1 : type) (t2 : type) : option value :=
+match v1, v2, t1, t2 with 
+| Vunit, Vunit, (Ptype Tunit), (Ptype Tunit)  => None
+| Vbool b1, Vbool b2, (Ptype Tbool), (Ptype Tbool) => None 
+| Vint i1, Vint i2, (Ptype Tint), (Ptype Tint) => 
+                      if (Int.eq i2 Int.zero) || (Int.eq i1 (Int.repr Int.min_signed) && Int.eq i2 Int.mone) (* -128/-1 *)
                       then None 
                       else Some (of_int (Int.divs i1 i2))
-| Vuint i1, Vuint i2 => if (Int.eq i2 Int.zero) then None else Some (of_int (Int.divu i1 i2)) 
-| Vloc l1, Vloc l2 => None 
-| _, _ => None
+| Vuint i1, Vuint i2, (Ptype Tunit), (Ptype Tunit) => if (Int.eq i2 Int.zero) then None else Some (of_int (Int.divu i1 i2)) 
+| Vloc l1, Vloc l2, (Reftype _ (Bprim Tint)), (Reftype _ (Bprim Tint)) => None 
+| _, _, _, _ => None
 end.
 
-Definition sem_and (v1 : value) (v2 : value) : option value :=
-match v1, v2 with 
-| Vunit, Vunit => None
-| Vbool b1, Vbool b2 => Some (of_bool (b1 && b2)) 
-| Vint i1, Vint i2 => None 
-| Vuint i1, Vuint i2 => None
-| Vloc l1, Vloc l2 => None 
-| _, _ => None
+Definition sem_and (v1 : value) (v2 : value) (t1 : type) (t2 : type) : option value :=
+match v1, v2, t1, t2 with 
+| Vunit, Vunit, (Ptype Tunit), (Ptype Tunit) => None
+| Vbool b1, Vbool b2, (Ptype Tbool), (Ptype Tbool) => Some (of_bool (b1 && b2)) 
+| Vint i1, Vint i2, (Ptype Tint), (Ptype Tint) => None 
+| Vuint i1, Vuint i2, (Ptype Tuint), (Ptype Tuint) => None
+| Vloc l1, Vloc l2, (Reftype _ (Bprim Tint)), (Reftype _ (Bprim Tint)) => None 
+| _, _, _, _ => None
 end.
 
-Definition sem_or (v1 : value) (v2 : value) : option value :=
-match v1, v2 with 
-| Vunit, Vunit => None
-| Vbool b1, Vbool b2 => Some (of_bool (b1 || b2)) 
-| Vint i1, Vint i2 => None 
-| Vuint i1, Vuint i2 => None
-| Vloc l1, Vloc l2 => None 
-| _, _ => None
+Definition sem_or (v1 : value) (v2 : value) (t1 : type) (t2 : type) : option value :=
+match v1, v2, t1, t2 with 
+| Vunit, Vunit, (Ptype Tunit), (Ptype Tunit) => None
+| Vbool b1, Vbool b2, (Ptype Tbool), (Ptype Tbool) => Some (of_bool (b1 || b2)) 
+| Vint i1, Vint i2, (Ptype Tint), (Ptype Tint) => None 
+| Vuint i1, Vuint i2, (Ptype Tuint), (Ptype Tuint)  => None
+| Vloc l1, Vloc l2, (Reftype _ (Bprim Tint)), (Reftype _ (Bprim Tint)) => None 
+| _, _, _, _ => None
 end.
 
-Definition sem_xor (v1 : value) (v2 : value) : option value :=
-match v1, v2 with 
-| Vunit, Vunit => None
-| Vbool b1, Vbool b2 => Some (of_bool (xorb b1 b2)) 
-| Vint i1, Vint i2 => None 
-| Vuint i1, Vuint i2 => None
-| Vloc l1, Vloc l2 => None 
-| _, _ => None
+Definition sem_xor (v1 : value) (v2 : value) (t1 : type) (t2 : type) : option value :=
+match v1, v2, t1, t2 with 
+| Vunit, Vunit, (Ptype Tunit), (Ptype Tunit) => None
+| Vbool b1, Vbool b2, (Ptype Tbool), (Ptype Tbool) => Some (of_bool (xorb b1 b2)) 
+| Vint i1, Vint i2, (Ptype Tint), (Ptype Tint) => None 
+| Vuint i1, Vuint i2, (Ptype Tuint), (Ptype Tuint)  => None
+| Vloc l1, Vloc l2, (Reftype _ (Bprim Tint)), (Reftype _ (Bprim Tint)) => None 
+| _, _, _, _ => None
 end.
 
-Definition sem_shl (v1 : value) (v2 : value) : option value :=
-match v1, v2 with 
-| Vunit, Vunit => None
-| Vbool b1, Vbool b2 => None
-| Vint i1, Vint i2 => Some (of_int (Int.shl i1 i2))
-| Vuint i1, Vuint i2 => Some (of_int (Int.shl i1 i2))
-| Vloc l1, Vloc l2 => None 
-| _, _ => None
+Definition sem_shl (v1 : value) (v2 : value) (t1 : type) (t2 : type) : option value :=
+match v1, v2, t1, t2 with 
+| Vunit, Vunit, (Ptype Tunit), (Ptype Tunit) => None
+| Vbool b1, Vbool b2, (Ptype Tbool), (Ptype Tbool) => None
+| Vint i1, Vint i2, (Ptype Tint), (Ptype Tint) => Some (of_int (Int.shl i1 i2))
+| Vuint i1, Vuint i2, (Ptype Tuint), (Ptype Tuint) => Some (of_int (Int.shl i1 i2))
+| Vloc l1, Vloc l2, (Reftype _ (Bprim Tint)), (Reftype _ (Bprim Tint)) => None 
+| _, _, _, _ => None
 end.
 
-Definition sem_shr (v1 : value) (v2 : value) : option value :=
-match v1, v2 with 
-| Vunit, Vunit => None
-| Vbool b1, Vbool b2 => None
-| Vint i1, Vint i2 => Some (of_int (Int.shr i1 i2))
-| Vuint i1, Vuint i2 => Some (of_int (Int.shru i1 i2))
-| Vloc l1, Vloc l2 => None 
-| _, _ => None
+Definition sem_shr (v1 : value) (v2 : value) (t1 : type) (t2 : type) : option value :=
+match v1, v2, t1, t2 with 
+| Vunit, Vunit, (Ptype Tunit), (Ptype Tunit) => None
+| Vbool b1, Vbool b2, (Ptype Tbool), (Ptype Tbool) => None
+| Vint i1, Vint i2, (Ptype Tint), (Ptype Tint) => Some (of_int (Int.shr i1 i2))
+| Vuint i1, Vuint i2, (Ptype Tuint), (Ptype Tuint) => Some (of_int (Int.shru i1 i2))
+| Vloc l1, Vloc l2, (Reftype _ (Bprim Tint)), (Reftype _ (Bprim Tint)) => None 
+| _, _, _, _ => None
 end.
 
-Definition sem_eq (v1 : value) (v2 : value) : option value :=
-match v1, v2 with 
-| Vunit, Vunit => Some (Vbool true)
-| Vbool b1, Vbool b2 => Some (of_bool (Bool.eqb b1 b2))
-| Vint i1, Vint i2 => Some (of_bool (Int.cmp Ceq i1 i2))
-| Vuint i1, Vuint i2 => Some (of_bool (Int.cmpu Ceq i1 i2))
-| Vloc l1, Vloc l2 => Some (of_bool (l1 =? l2)%positive) 
-| _, _ => None
+Definition sem_eq (v1 : value) (v2 : value) (t1 : type) (t2 : type) : option value :=
+match v1, v2, t1, t2 with 
+| Vunit, Vunit, (Ptype Tunit), (Ptype Tunit) => Some (Vbool true)
+| Vbool b1, Vbool b2, (Ptype Tbool), (Ptype Tbool) => Some (of_bool (Bool.eqb b1 b2))
+| Vint i1, Vint i2, (Ptype Tint), (Ptype Tint) => Some (of_bool (Int.cmp Ceq i1 i2))
+| Vuint i1, Vuint i2, (Ptype Tuint), (Ptype Tuint) => Some (of_bool (Int.cmpu Ceq i1 i2))
+| Vloc l1, Vloc l2, (Reftype _ (Bprim Tint)), (Reftype _ (Bprim Tint))  => Some (of_bool (l1 =? l2)%positive) 
+| _, _, _, _ => None
 end.
 
-Definition sem_neq (v1 : value) (v2 : value) : option value :=
-match v1, v2 with 
-| Vunit, Vunit => Some (Vbool true)
-| Vbool b1, Vbool b2 => Some (of_bool (Bool.eqb b1 b2))
-| Vint i1, Vint i2 => Some (of_bool (Int.cmp Cne i1 i2))
-| Vuint i1, Vuint i2 => Some (of_bool (Int.cmpu Cne i1 i2))
-| Vloc l1, Vloc l2 => Some (of_bool (negb (l1 =? l2)%positive)) 
-| _, _ => None
+Definition sem_neq (v1 : value) (v2 : value) (t1 : type) (t2 : type) : option value :=
+match v1, v2, t1, t2 with 
+| Vunit, Vunit, (Ptype Tunit), (Ptype Tunit) => Some (Vbool true)
+| Vbool b1, Vbool b2, (Ptype Tbool), (Ptype Tbool) => Some (of_bool (Bool.eqb b1 b2))
+| Vint i1, Vint i2, (Ptype Tint), (Ptype Tint) => Some (of_bool (Int.cmp Cne i1 i2))
+| Vuint i1, Vuint i2, (Ptype Tuint), (Ptype Tuint) => Some (of_bool (Int.cmpu Cne i1 i2))
+| Vloc l1, Vloc l2, (Reftype _ (Bprim Tint)), (Reftype _ (Bprim Tint))  => Some (of_bool (negb (l1 =? l2)%positive)) 
+| _, _, _, _ => None
 end.
 
-Definition sem_lt (v1 : value) (v2 : value) : option value :=
-match v1, v2 with 
-| Vunit, Vunit => None
-| Vbool b1, Vbool b2 => None
-| Vint i1, Vint i2 => Some (of_bool (Int.cmp Clt i1 i2))
-| Vuint i1, Vuint i2 => Some (of_bool (Int.cmpu Clt i1 i2))
-| Vloc l1, Vloc l2 => None
-| _, _ => None
+Definition sem_lt (v1 : value) (v2 : value) (t1 : type) (t2 : type) : option value :=
+match v1, v2, t1, t2 with 
+| Vunit, Vunit, (Ptype Tunit), (Ptype Tunit) => Some (Vbool true)
+| Vbool b1, Vbool b2, (Ptype Tbool), (Ptype Tbool) => None
+| Vint i1, Vint i2, (Ptype Tint), (Ptype Tint) => Some (of_bool (Int.cmp Clt i1 i2))
+| Vuint i1, Vuint i2, (Ptype Tuint), (Ptype Tuint) => Some (of_bool (Int.cmpu Clt i1 i2))
+| Vloc l1, Vloc l2, (Reftype _ (Bprim Tint)), (Reftype _ (Bprim Tint))  => None 
+| _, _, _, _ => None
 end.
 
-Definition sem_lte (v1 : value) (v2 : value) : option value :=
-match v1, v2 with 
-| Vunit, Vunit => None
-| Vbool b1, Vbool b2 => None
-| Vint i1, Vint i2 => Some (of_bool (Int.cmp Cle i1 i2))
-| Vuint i1, Vuint i2 => Some (of_bool (Int.cmpu Cle i1 i2))
-| Vloc l1, Vloc l2 => None
-| _, _ => None
+Definition sem_lte (v1 : value) (v2 : value) (t1 : type) (t2 : type) : option value :=
+match v1, v2, t1, t2 with 
+| Vunit, Vunit, (Ptype Tunit), (Ptype Tunit) => Some (Vbool true)
+| Vbool b1, Vbool b2, (Ptype Tbool), (Ptype Tbool) => None
+| Vint i1, Vint i2, (Ptype Tint), (Ptype Tint) => Some (of_bool (Int.cmp Cle i1 i2))
+| Vuint i1, Vuint i2, (Ptype Tuint), (Ptype Tuint) => Some (of_bool (Int.cmpu Cle i1 i2))
+| Vloc l1, Vloc l2, (Reftype _ (Bprim Tint)), (Reftype _ (Bprim Tint))  => None 
+| _, _, _, _ => None
 end.
 
-Definition sem_gt (v1 : value) (v2 : value) : option value :=
-match v1, v2 with 
-| Vunit, Vunit => None
-| Vbool b1, Vbool b2 => None
-| Vint i1, Vint i2 => Some (of_bool (Int.cmp Cgt i1 i2))
-| Vuint i1, Vuint i2 => Some (of_bool (Int.cmpu Cgt i1 i2))
-| Vloc l1, Vloc l2 => None
-| _, _ => None
+Definition sem_gt (v1 : value) (v2 : value) (t1 : type) (t2 : type) : option value :=
+match v1, v2, t1, t2 with 
+| Vunit, Vunit, (Ptype Tunit), (Ptype Tunit) => Some (Vbool true)
+| Vbool b1, Vbool b2, (Ptype Tbool), (Ptype Tbool) => None
+| Vint i1, Vint i2, (Ptype Tint), (Ptype Tint) => Some (of_bool (Int.cmp Cgt i1 i2))
+| Vuint i1, Vuint i2, (Ptype Tuint), (Ptype Tuint) => Some (of_bool (Int.cmpu Cgt i1 i2))
+| Vloc l1, Vloc l2, (Reftype _ (Bprim Tint)), (Reftype _ (Bprim Tint))  => None 
+| _, _, _, _ => None
 end.
 
-Definition sem_gte (v1 : value) (v2 : value) : option value :=
-match v1, v2 with 
-| Vunit, Vunit => None
-| Vbool b1, Vbool b2 => None
-| Vint i1, Vint i2 => Some (of_bool (Int.cmp Cge i1 i2))
-| Vuint i1, Vuint i2 => Some (of_bool (Int.cmpu Cge i1 i2))
-| Vloc l1, Vloc l2 => None
-| _, _ => None
+Definition sem_gte (v1 : value) (v2 : value) (t1 : type) (t2 : type) : option value :=
+match v1, v2, t1, t2 with 
+| Vunit, Vunit, (Ptype Tunit), (Ptype Tunit) => Some (Vbool true)
+| Vbool b1, Vbool b2, (Ptype Tbool), (Ptype Tbool) => None
+| Vint i1, Vint i2, (Ptype Tint), (Ptype Tint) => Some (of_bool (Int.cmp Cge i1 i2))
+| Vuint i1, Vuint i2, (Ptype Tuint), (Ptype Tuint) => Some (of_bool (Int.cmpu Cge i1 i2))
+| Vloc l1, Vloc l2, (Reftype _ (Bprim Tint)), (Reftype _ (Bprim Tint))  => None 
+| _, _, _, _ => None
 end.
 
-Definition sem_binary_operation (op : bop) (v1 v2 : value) : option value :=
+Definition sem_binary_operation (op : bop) (v1 v2 : value) (t1 t2 : type) : option value :=
 match op with 
-| Plus => sem_plus v1 v2
-| Minus => sem_minus v1 v2
-| Mult => sem_mult v1 v2
-| Div => sem_div v1 v2
-| And => sem_and v1 v2
-| Or => sem_or v1 v2
-| Xor => sem_xor v1 v2
-| Shl => sem_shl v1 v2
-| Shr => sem_shr v1 v2
-| Eq => sem_eq v1 v2
-| Neq => sem_neq v1 v2
-| Lt => sem_lt v1 v2
-| Lte => sem_lte v1 v2
-| Gt => sem_gt v1 v2
-| Gte => sem_gte v1 v2
+| Plus => sem_plus v1 v2 t1 t2
+| Minus => sem_minus v1 v2 t1 t2
+| Mult => sem_mult v1 v2 t1 t2
+| Div => sem_div v1 v2 t1 t2
+| And => sem_and v1 v2 t1 t2
+| Or => sem_or v1 v2 t1 t2
+| Xor => sem_xor v1 v2 t1 t2
+| Shl => sem_shl v1 v2 t1 t2
+| Shr => sem_shr v1 v2 t1 t2
+| Eq => sem_eq v1 v2 t1 t2
+| Neq => sem_neq v1 v2 t1 t2
+| Lt => sem_lt v1 v2 t1 t2
+| Lte => sem_lte v1 v2 t1 t2
+| Gt => sem_gt v1 v2 t1 t2
+| Gte => sem_gte v1 v2 t1 t2
 end.
 
 (* Operational Semantics *) 
@@ -405,43 +408,43 @@ Inductive sem_expr : genv -> state -> expr -> state -> value -> Prop :=
              sem_expr ge st e st' (Vloc l) ->
              get_fun_decl ge l = Some (Fdecl fd) ->
              sem_exprs ge st' es st'' vs ->
-             typeof_values vs = unzip2 (fd.(args)) ->
+             typeof_values vs (unzip2 (fd.(args))) ->
              write_vars (st.(vmem)) (unzip1 fd.(args)) vs = Ok error vm' ->
              sem_expr ge {| hmem := st''.(hmem); vmem := vm' |} fd.(body) st''' rv -> 
              write_var (st'''.(vmem)) r rv = vm'' ->
-             typeof_value rv = fd.(rtype) ->
+             typeof_value rv (fd.(rtype)) ->
              sem_expr ge st (App (Some r) e es t) {| hmem := st'''.(hmem); vmem := vm'' |}  rv 
 | sem_app : forall ge e es t st l st' st'' vs fd vm' st''' rv vm'',
              sem_expr ge st e st' (Vloc l) ->
              get_fun_decl ge l = Some (Fdecl fd) ->
              sem_exprs ge st' es st'' vs ->
-             typeof_values vs = unzip2 (fd.(args)) ->
+             typeof_values vs (unzip2 (fd.(args))) ->
              write_vars (st.(vmem)) (unzip1 fd.(args)) vs = Ok error vm' ->
              sem_expr ge {| hmem := st''.(hmem); vmem := vm' |} fd.(body) st''' rv -> 
-             typeof_value rv = fd.(rtype) ->
+             typeof_value rv (fd.(rtype)) ->
              sem_expr ge st (App None e es t) {| hmem := st'''.(hmem); vmem := vm'' |}  rv 
 | sem_prim_uop : forall ge st e t v uop st' v',
                  sem_expr ge st e st' v ->
-                 sem_unary_operation uop v = Some v' ->
-                 typeof_expr e = typeof_value v ->
+                 sem_unary_operation uop v (typeof_expr e) = Some v' ->
+                 typeof_value v (typeof_expr e) ->
                  sem_expr ge st (Prim (Uop uop) (e :: nil) t) st' v'
 | sem_prim_bop : forall ge st e1 e2 t v1 v2 bop st' st'' v,
                  sem_expr ge st e1 st' v1 ->
                  sem_expr ge st' e2 st'' v2 ->
-                 sem_binary_operation bop v1 v2 = Some v ->
-                 typeof_expr e1 = typeof_value v1 ->
-                 typeof_expr e2 = typeof_value v2 ->
+                 sem_binary_operation bop v1 v2 (typeof_expr e1) (typeof_expr e2) = Some v ->
+                 typeof_value v1 (typeof_expr e1) ->
+                 typeof_value v2 (typeof_expr e2) ->
                  sem_expr ge st (Prim (Bop bop) (e1 :: e2 :: nil) t) st' v
 | sem_prim_ref : forall ge st e t l st' h v, 
                  sem_expr ge st e st' v ->
                  fresh_loc st'.(hmem) l = true ->
                  update_heap st'.(hmem) l v = h ->
-                 typeof_value v = typeof_expr e ->
+                 typeof_value v (typeof_expr e) ->
                  sem_expr ge st (Prim Deref (e :: nil) t) st' v
 | sem_prim_deref : forall ge st e t l st' v, 
                    sem_expr ge st e st' (Vloc l) ->
                    get_val_loc st.(hmem) l = Some v -> 
-                   typeof_value v = typeof_expr e ->
+                   typeof_value v (typeof_expr e) ->
                    sem_expr ge st (Prim Deref (e :: nil) t) st' v
 | sem_prim_massgn : forall ge st e1 e2 t l v h st' st'',
                     sem_expr ge st e1 st' (Vloc l) -> 
